lean/Sable.lean
@@ -9,3 +9,4 @@ import Sable.Perm
 import Sable.Specs
 import Sable.SVM
 import Sable.SVMEval
+import Sable.SVMRawTests
